% !TEX program = lualatex
\documentclass{article}
 \usepackage[T1]{fontenc}
 \newcommand{\diff}{\mathop{}\!d}
 % For italic
 % \newcommand{\diff}{\mathop{}\!\mathrm{d}} % For upright
\usepackage{amsmath}
\usepackage{bm}
\usepackage{mathtools}
 \begin{document}
 A sentence with inline mathematics: $y = mx + c$.

 A second sentence with inline mathematics:
 \(5^{2}=3^{2}+4^{2}\).
 
A second paragraph containing display math.
 \[
 y = mx + c
 \]
 See how the paragraph continues after the display.

Number without math 2y+10x.

Superscripts $a^{b}$ and subscripts $a_{b}$.

Some mathematics: $y = 2 \sin \theta^{2}$.

A paragraph about a larger equation
 \[
 \int_{-\infty}^{+\infty} e^{-x^2} \, dx
 \]

 A paragraph about a larger equation with diff
 \[
 \int_{-\infty}^{+\infty} e^{-x^2} \diff x
 \]

A paragraph about a larger equation with numberedequation
 \begin{equation}
 \int_{-\infty}^{+\infty} e^{-x^2} \, dx
 \end{equation}

Solve the following recurrence for $ n,k\geq 0 $:
 \begin{align*}
 Q_{n,0} &= 1 \quad Q_{0,k} = [k=0]; \\
 Q_{n,k} &= Q_{n-1,k}+Q_{n-1,k-1}+\binom{n}{k}, \quad\text{for $n$, $k>0$.}
 \end{align*}

AMS matrices.
 \[
 \begin{matrix}
 a & b & c \\
 d & e & f
 \end{matrix}
 \quad
 \begin{pmatrix}
 a & b & c \\
 d & e & f
 \end{pmatrix}
 \quad
 \begin{bmatrix}
 a & b & c \\
 d & e & f
 \end{bmatrix}
 \]

Fonts in math mode: The matrix $\mathbf{M}$. The matrix $\mathit{M}$.

$\text{bad use } size \neq \mathit{size} \neq \mathrm{size} $

\textit{$\text{bad use } size \neq \mathit{size} \neq \mathrm{size} $}

Gather
 \begin{gather}
 P(x)=ax^{5}+bx^{4}+cx^{3}+dx^{2}+ex +f\\
 x^2+x=10
 \end{gather}
 Multline
 \begin{multline*}
 (a+b+c+d)x^{5}+(b+c+d+e)x^{4} \\
 +(c+d+e+f)x^{3}+(d+e+f+a)x^{2}+(e+f+a+b)x\\
 + (f+a+b+c)
 \end{multline*}

 Aligned equations
 \begin{align*}
 a &= b+1 & c &= d+2 & e &= f+3 \\
 r &= s^{2} & t &=u^{3} & v &= w^{4}
 \end{align*}

 \begin{itemize}
 \item
 $\begin{aligned}[t]
 a&=b\\
 c&=d
 \end{aligned}$
 \item
 $\begin{aligned}
 a&=b\\
 c&=d
 \end{aligned}$
 \end{itemize}

$(x+y)(x-y)=x^{2}-y^{2}$

 {\boldmath $(x+y)(x-y)=x^{2}-y^{2}$ $\pi r^2$}

 $(x+\mathbf{y})(x-\mathbf{y})=x^{2}-{\mathbf{y}}^{2}$

 $\mathbf{\pi} r^2$ % bad use of \mathbf

 $(x+\mathbf{y})(x-\mathbf{y})=x^{2}-{\mathbf{y}}^{2}$

 $(x+\bm{y})(x-\bm{y}) \bm{=} x^{2}-{\bm{y}}^{2}$

 $\alpha + \bm{\alpha} < \beta + \bm{\beta}$

\[
 \begin{pmatrix*}[r]
 10&11\\
 1&2\\-5&-6
 \end{pmatrix*}
 \]

 \end{document}